Demote V to a definition

src/Codes.v
@@ -21,8 +21,7 @@ Inductive code {Var : Set} : Set :=
   | code_b : code
   | code_c : code
   | code_s : code
-  | code_y : code
-  | code_v : code.
+  | code_y : code.
 Hint Constructors code.
 Definition Code (Var : Set) := @code Var.
 
@@ -42,7 +41,6 @@ Notation "'B'" := code_b : code_scope.
 Notation "'C'" := code_c : code_scope.
 Notation "'S'" := code_s : code_scope.
 Notation "'Y'" := code_y : code_scope.
-Notation "'V'" := code_v : code_scope.
 Notation "x 'o' y" := (code_b * x * y)%code : code_scope.
 Notation "x || y" := (code_j * x * y)%code : code_scope.
 Notation "x (+) y" := (code_r * x * y)%code : code_scope.
@@ -61,7 +59,6 @@ Inductive beta {Var : Set} : Code Var -> Code Var -> Prop :=
   | beta_c {x y z} : beta (C * x * y * z) (x * z * y)
   | beta_s {x y z} : beta (S * x * y * z) (x * z * (y * z))
   | beta_y {x} : beta (Y * x) (x * (Y * x))
-  | beta_v {x} : beta (V * x) (I || x o (V * x))
   | beta_j_ap {x y z} : beta ((x || y) * z) (x * z || y * z)
   | beta_r_ap {x y z} : beta ((x (+) y) * z) (x * z (+) y * z)
   | beta_r_idem {x} : beta (x (+) x) x
@@ -91,14 +88,13 @@ Definition Beta_b (Var : Set) := (@beta_b Var).
 Definition Beta_c (Var : Set) := (@beta_c Var).
 Definition Beta_s (Var : Set) := (@beta_s Var).
 Definition Beta_y (Var : Set) := (@beta_y Var).
-Definition Beta_v (Var : Set) := (@beta_v Var).
 Definition Beta_j_ap (Var : Set) := (@beta_j_ap Var).
 Definition Beta_r_ap (Var : Set) := (@beta_r_ap Var).
 Definition Beta_r_idem (Var : Set) := (@beta_r_idem Var).
 
 Hint Rewrite Beta_i Beta_k Beta_b Beta_c Beta_j_ap Beta_r_ap Beta_r_idem
   : beta_safe.
-Hint Rewrite Beta_s Beta_y Beta_v
+Hint Rewrite Beta_s Beta_y
   : beta_unsafe.
 
 Tactic Notation "beta_simpl" := autorewrite with beta_safe.
@@ -239,45 +235,6 @@ Proof.
   reflexivity.
 Qed.
 
-Definition div {Var : Set} : Code Var := V * (C * I * TOP).
-
-Lemma beta_div (Var : Set) (x : Code Var) :
-  beta (div * x) (x || div * x * TOP).
-Proof.
-  unfold div.
-  rewrite beta_v at 1; beta_simpl; auto.
-Qed.
-
-Definition conv {Var : Set} (x : Code Var) := approx (div * x) TOP.
-
-Lemma conv_top (Var : Set) : conv (TOP : Code Var).
-Proof.
-  unfold conv; rewrite beta_div; rewrite pi_j_left; reflexivity.
-Qed.
-Hint Resolve conv_top.
-
-Instance conv_beta (Var : Set) : Proper (beta ==> iff) (@conv Var).
-Proof.
-  compute; intros x x' Hx; split; intros Hc;
-  inversion Hc as [u v w]; apply approx_intro with v; auto.
-    rewrite <- Hx; auto.
-  rewrite -> Hx; auto.
-Qed.
-
-Instance conv_pi (Var : Set) : Proper (pi --> impl) (@conv Var).
-Proof.
-  compute; intros x x' xx' Ha.
-  rewrite xx'; auto.
-Qed.
-
-Inductive prob {Var : Set} : Code Var -> Prop :=
-  | prob_top : prob TOP
-  | prob_bot : prob BOT
-  | prob_r p q : prob p -> prob q -> prob (p (+) q).
-
-Definition pconv {Var : Set} (x : Code Var) (p : Code Var) :=
-  approx (div * x) p.
-
 (** ** Substitution *)
 
 Fixpoint code_sub {Var Var' : Set}
@@ -295,7 +252,6 @@ Fixpoint code_sub {Var Var' : Set}
   | C => C
   | S => S
   | Y => Y
-  | V => V
   end.
 
 Notation "x @ f" := (code_sub f x)%code : code_scope.
@@ -456,7 +412,6 @@ Fixpoint code_abs {Var Var' : Set} (b : Var -> option Var') (x : Code Var) :
   | C => K * C
   | S => K * S
   | Y => K * Y
-  | V => K * V
   end.
 
 Section beta_abs_sub.
@@ -507,3 +462,59 @@ Definition code_lambda {Var : Set} (x y : Code (nat + Var)) :
   end.
 
 Notation "\ x , y" := (code_lambda x y)%code : code_scope.
+
+(** ** Convergence testing *)
+
+Section V.
+  Context {Var : Set}.
+  Let a := make_var Var 0.
+  Let x := make_var Var 1.
+  Definition V := Eval compute in close
+    (\a, Y * \x, I || a o x).
+End V.
+
+Lemma beta_v (Var : Set) (a : Code Var) : beta (V * a) (I || a o (V * a)).
+Proof.
+  unfold V; beta_simpl; rewrite beta_y at 1; beta_simpl; auto.
+Qed.
+Hint Rewrite beta_v : beta_unsafe.
+
+Definition div {Var : Set} : Code Var := V * (C * I * TOP).
+
+Lemma beta_div (Var : Set) (x : Code Var) :
+  beta (div * x) (x || div * x * TOP).
+Proof.
+  unfold div.
+  rewrite beta_v at 1; beta_simpl; auto.
+Qed.
+
+Definition conv {Var : Set} (x : Code Var) := approx (div * x) TOP.
+
+Lemma conv_top (Var : Set) : conv (TOP : Code Var).
+Proof.
+  unfold conv; rewrite beta_div; rewrite pi_j_left; reflexivity.
+Qed.
+Hint Resolve conv_top.
+
+Instance conv_beta (Var : Set) : Proper (beta ==> iff) (@conv Var).
+Proof.
+  compute; intros x x' Hx; split; intros Hc;
+  inversion Hc as [u v w]; apply approx_intro with v; auto.
+    rewrite <- Hx; auto.
+  rewrite -> Hx; auto.
+Qed.
+
+Instance conv_pi (Var : Set) : Proper (pi --> impl) (@conv Var).
+Proof.
+  compute; intros x x' xx' Ha.
+  rewrite xx'; auto.
+Qed.
+
+Inductive prob {Var : Set} : Code Var -> Prop :=
+  | prob_top : prob TOP
+  | prob_bot : prob BOT
+  | prob_r p q : prob p -> prob q -> prob (p (+) q).
+
+Definition pconv {Var : Set} (x : Code Var) (p : Code Var) :=
+  approx (div * x) p.
+
